Transplant to typing done.

src/SmallCoreTyping.v
@@ -8,8 +8,10 @@ Require Import LibTactics.
 Require Import SmallCore.
 Require Import Coq.ZArith.ZArith.
 Require Import SmallCorePropSubty.
+Require Import SmallCoreStep.
 
 Import SmallCore.SmallCore.
+Import SmallCoreStep.SmallCoreStep.
 Import SmallCorePropSubty.SmallCorePropSubty.
 Import Context.Context.
 
@@ -68,4 +70,310 @@ Inductive has_type : Context (type := {x : ty | wf_ty x}) -> tm -> ty -> Prop :=
 
 Hint Constructors has_type.
 
-End SmallCoreTyping.
+
+Inductive free_occur_in : id -> tm -> Prop :=
+    | fo_rcons0 : forall i j t0 t1,
+                free_occur_in i t0 ->
+                free_occur_in i (trcons j t0 t1)
+    | fo_rcons1 : forall i j t0 t1,
+                free_occur_in i t1 ->
+                free_occur_in i (trcons j t0 t1)
+    | fo_var : forall i,
+                free_occur_in i (tvar i)
+
+    | fo_fun : forall i j T h body,
+                i <> j ->
+                free_occur_in i body ->
+                free_occur_in i (tfun j T h body)
+    | fo_app0 : forall i t0 t1,
+                free_occur_in i t0 ->
+                free_occur_in i (tapp t0 t1)
+    | fo_app1 : forall i t0 t1,
+                free_occur_in i t1 ->
+                free_occur_in i (tapp t0 t1)
+    | fo_let0 : forall i j T h t0 t1,
+                free_occur_in i t0 ->
+                free_occur_in i (tlet j T h t0 t1)
+    | fo_let1 : forall i j T h t0 t1,
+                i <> j ->
+                free_occur_in i t1 ->
+                free_occur_in i (tlet j T h t0 t1)
+    | fo_fixApp : forall i j T h t0,
+                i <> j ->
+                free_occur_in i t0 ->
+                free_occur_in i (tfixApp j T h t0)
+    | fo_left : forall i t0 T h,
+                free_occur_in i t0 ->
+                free_occur_in i (tleft t0 T h)
+    | fo_right: forall i t0 T h,
+                free_occur_in i t0 ->
+                free_occur_in i (tright T h t0)
+    | fo_case0: forall i t0 t1 t2,
+                free_occur_in i t0 ->
+                free_occur_in i (tcase t0 t1 t2)
+    | fo_case1: forall i t0 t1 t2,
+                free_occur_in i t1 ->
+                free_occur_in i (tcase t0 t1 t2)
+    | fo_case2: forall i t0 t1 t2,
+                free_occur_in i t2 ->
+                free_occur_in i (tcase t0 t1 t2).
+
+Hint Constructors free_occur_in.
+        
+(*Lemma closed_no_free_occur:
+    forall t T,
+        has_type empty t T ->
+        forall i, ~ free_occur_in i t.
+    intros t T h0.
+    remember empty as ctx0.
+    glize Heqctx0 0.
+    induction h0; intros; subst; intro; 
+    repeat (
+        match goal with
+        | h : ?x = ?x -> _ |- _ => poses' (h eq_refl); clear h
+        end
+    );
+    try (
+    repeat (
+        match goal with
+        | h : forall _ : id, _ |- _ => poses' (h i); glize h 0
+        end); 
+    intros;
+    try match goal with
+    | h1 : free_occur_in _ _ |- _ => inversion h1; subst; eauto; fail
+    | h1 : free_occur_in _ _ |- _ => inversion h1; subst;
+        match goal with
+        | h2 : free_occur_in ?ii ?t, h3: forall _:id, ~free_occur_in _ ?t |- _ => 
+            poses' (h3 ii); eauto
+        end; fail 
+    end; 
+    fail
+    ).
+
+    (* case tvar *)
+    cbn in H. inversion H.
+    (* case tfun *)
+    inversion H; subst; eauto.  
+    Abort.
+    *)
+Definition relative_ctx_eq (t : tm) (ctx0 ctx1: Context) :=
+    (forall i, free_occur_in i t ->  
+                byContext (type := {x : ty | wf_ty x}) ctx0 i = byContext ctx1 i).
+
+Theorem rce_refl:
+    forall t x,
+    relative_ctx_eq t x x.
+    unfold relative_ctx_eq.
+    eauto.
+Qed.
+
+Theorem rce_symm:
+    forall t x y,
+        relative_ctx_eq t x y ->
+        relative_ctx_eq t y x.
+    unfold relative_ctx_eq.
+    intros; eauto. symmetry. eauto.
+Qed.
+
+Theorem rce_trans:
+    forall t x y z,
+        relative_ctx_eq t x y ->
+        relative_ctx_eq t y z ->
+        relative_ctx_eq t x z.
+    unfold relative_ctx_eq.
+    intros. poses' (H _ H1); poses' (H0 _ H1).
+    rewrite H2; rewrite H3.
+    auto.
+Qed.
+    
+Hint Unfold relative_ctx_eq.
+
+
+
+Theorem ctx_change:
+    forall ctx0 ctx1 t T,
+    has_type ctx0 t T ->
+    relative_ctx_eq t ctx0 ctx1 ->
+    has_type ctx1 t T.
+
+    intros ctx0 ctx1 t T h0. glize ctx1 0.
+    unfold relative_ctx_eq.
+    induction h0; intros; subst; eauto;
+    try(
+    repeat (
+        match goal with
+        | h1: forall _: Context, _ |- _ => poses' (h1 ctx1); glize h1 0
+        end
+    );
+    intros;
+    repeat (
+        match goal with
+        | h0 :  _ -> has_type _ _ _ |- _ => forwards: h0; glize h0 0
+        end
+    );
+    intros;
+    eauto;
+    fail).
+
+    (* case tvar*)
+    poses' (H0 i). forwards: H1; eauto.
+    pattern (byContext ctx i) in H.
+    rewrite H2 in H. eauto.
+
+    (* case tfun*)
+    eapply ht_fun.
+    eapply IHh0. 
+    intros. cbn. destruct (eq_id_dec i0 i); subst; eauto.
+
+    (* case tlet*)
+    eapply ht_let. eapply IHh0_1.
+    intros. eauto.
+    eapply IHh0_2. intros; eauto.
+    cbn. destruct (eq_id_dec i0 i); subst; eauto.
+
+    (* case tfix *)
+    eapply ht_fix. eapply IHh0. intros; cbn.
+    destruct (eq_id_dec i0 i); subst; eauto.
+Qed.
+
+Lemma ctx_typed_fv_exists:
+    forall ctx t T,
+        has_type ctx t T ->
+        (forall i, free_occur_in i t -> exists h, byContext ctx i = Some h).
+
+    intros ctx t T h0.
+    induction h0 ; subst; eauto; intros;
+    try (
+        match goal with
+        | h: free_occur_in _ _ |- _ =>
+            inversion h; subst; eauto; fail
+        end
+    );
+    try (
+        (* Eliminate all cases that depends inductibly and no special cases *)
+    match goal with
+    | h : free_occur_in ?ii (_ _) |- _ => 
+            inversion h; subst; eauto;
+            
+                match goal with
+                | h : forall _:id, _ , h0 : free_occur_in ?ii _ |- _ -> _ =>
+                        destruct (h ii h0); glize h 0
+                end
+    end;
+    intros; eauto
+    ).
+    
+
+    (* case tfun *)
+    inversion H; subst; eauto.
+    destruct (IHh0 i0 H5); subst; eauto.
+    cbn in H0. destruct (eq_id_dec i0 i); subst; eauto; try contradiction.
+    
+    (* case tlet *)
+    inversion H; subst; eauto. destruct (IHh0_2 i0 H6); subst; eauto.
+    cbn in H0; subst; eauto. destruct (eq_id_dec i0 i); subst; eauto; try contradiction.
+
+    (* case tfix*)
+    inversion H; subst; eauto. destruct (IHh0 i0 H5); subst; eauto.
+    cbn in H0; subst; eauto. destruct (eq_id_dec i0 i); subst; eauto; try contradiction.
+
+Qed.
+
+
+Theorem typed_closed :
+    forall t T,
+        has_type empty t T ->
+        (forall i, ~ free_occur_in i t).
+
+    intros t T h0. remember empty as ctx0.
+    glize Heqctx0 0.
+    induction h0; intros; subst; intro;
+    repeat (
+        match goal with
+        | h : ?x = ?x -> _ |- _ => poses' (h eq_refl); clear h
+        end
+    );
+    try (
+        match goal with
+        | h : free_occur_in _ _ |- _ => 
+            inversion h; subst; eauto;
+            match goal with
+            | h0 : free_occur_in ?ii ?tt, h1 : forall _:id, ~ free_occur_in _ ?tt |- _ =>
+                destruct (h1 ii h0)
+            end
+        end; fail
+    ).
+
+    (* case tvar *)
+    inversion H.
+    (* case tfun*)
+    inversion H; subst; eauto.
+    destruct 
+    (ctx_typed_fv_exists 
+    (update i (exist wf_ty T h) empty) 
+    body TO h0 i0 H5).
+    cbn in H0. destruct (eq_id_dec i0 i); subst; eauto; try contradiction.
+    inversion H0.
+
+    (* case tlet *)
+    inversion H; subst; eauto.
+    destruct (H0 _ H3).
+    destruct 
+    (ctx_typed_fv_exists 
+    (update i (exist (fun x => wf_ty x) T h) empty)
+    body T' h0_2 i0 H7
+    ).
+    cbn in H1. destruct (eq_id_dec i0 i); subst; eauto; try contradiction.
+    inversion H1.
+
+    (* case tfix *)
+    inversion H; subst; eauto.
+    destruct 
+    (ctx_typed_fv_exists 
+    (update i (exist wf_ty T h) empty)
+    body T h0 i0 H5
+    ).
+    cbn in H0. destruct (eq_id_dec i0 i); subst; eauto; try contradiction.
+    inversion H0.
+Qed.
+
+
+
+
+Theorem typed_relative_closed:
+    forall t T,
+        has_type empty t T ->
+        forall ctx,
+            relative_ctx_eq t ctx empty.
+    intros t T h0.
+    poses' (typed_closed t T h0).
+    unfold relative_ctx_eq.
+    intros. destruct (H _ H0).
+Qed.
+
+Theorem ctx_eq_rewrite:
+    forall U V t T,
+        has_type U t T ->
+        CtxEq U V ->
+        has_type V t T.
+    intros U V t T h0;
+    glize V 0.
+    induction h0; subst; eauto.
+    intros. poses' (CtxEq_byCtxEq _ _ H0).
+    eapply ht_var. rewrite <- H1. eauto.
+Qed.
+
+
+Lemma empty_typed_ctx_typed:
+    forall t T,
+        has_type empty t T ->
+        forall ctx,
+            has_type ctx t T.
+    
+    intros t T h0 ctx.
+    poses' (typed_relative_closed _ _ h0 ctx) .
+    eapply ctx_change; eauto.
+    eapply rce_symm; eauto.
+Qed.
+
+
